Checkpoint before deleting some code

FMapExt.v
@@ -3,11 +3,63 @@ Require Import
   Coq.FSets.FMapFacts
   Coq.Structures.OrderedTypeEx.
 
+Lemma fold_right_filter : forall A B (f : A -> B -> B) z P l,
+  fold_right f z (filter P l) =
+  fold_right (fun x rest => if P x then f x rest else rest) z l.
+Proof.
+  intros.
+  induction l; simpl; trivial.
+  rewrite <- IHl; clear IHl.
+  destruct (P a); reflexivity.
+Qed.
+
 Module FMapExt (O : OrderedType).
 
 Module M := FMapList.Make(O).
 Module P := FMapFacts.Properties M.
 Module F := P.F.
+
+Ltac simplify_maps :=
+  match goal with
+  | [ H : M.find (elt:=?T) ?A (M.add ?K ?E ?M) = Some ?B |- _ ] =>
+    apply F.find_mapsto_iff, F.add_mapsto_iff in H;
+    let H1 := fresh "H1" in
+    let H2 := fresh "H2" in
+    let H3 := fresh "H3" in
+    let H4 := fresh "H4" in
+    destruct H as [[H1 H2]|[H3 H4]];
+    [subst|apply F.find_mapsto_iff in H4]
+  | [ H : M.find (elt:=?T) ?A (M.remove ?KE ?M) = Some ?B |- _ ] =>
+    apply F.find_mapsto_iff, F.remove_mapsto_iff in H;
+    let H1 := fresh "H1" in
+    let H2 := fresh "H2" in
+    destruct H as [H1 H2];
+    apply F.find_mapsto_iff in H2
+  | [ H : M.find (elt:=?T) ?A (M.map ?F ?M) = Some ?B |- _ ] =>
+    apply F.find_mapsto_iff, F.map_mapsto_iff in H;
+    let cblk := fresh "cblk" in
+    let H1 := fresh "H1" in
+    let H2 := fresh "H2" in
+    destruct H as [cblk [H1 H2]];
+    apply F.find_mapsto_iff in H2
+  | [ H : M.find (elt:=?T) ?A (P.filter ?F ?M) = Some ?B |- _ ] =>
+    apply F.find_mapsto_iff, P.filter_iff in H;
+    [let H1 := fresh "H1" in
+     let H2 := fresh "H2" in
+     destruct H as [H1 H2];
+     apply F.find_mapsto_iff in H1|]
+  | [ H : M.find (elt:=?T) ?A (M.mapi ?F ?M) = Some ?B |- _ ] =>
+    rewrite F.mapi_o, <- F.map_o in H
+  | [ H : M.find (elt:=?T) ?A (M.empty ?U) = Some ?B |- _ ] =>
+    apply F.find_mapsto_iff, F.empty_mapsto_iff in H;
+    contradiction
+  | [ H1 : M.find (elt:=?T) ?A ?M = Some ?B,
+      H2 : M.Empty (elt:=?T) ?M |- _ ] =>
+    apply P.elements_Empty in H2;
+    rewrite F.elements_o in H1;
+    rewrite H2 in H1;
+    inversion H1
+  end.
 
 Section for_all.
 
@@ -58,14 +110,15 @@ Proof.
   - tauto.
 Qed.
 
-Lemma mapi_empty (Oeq_eq : forall a b, O.eq a b -> a = b) :
+Lemma mapi_empty :
   forall (f : M.key -> elt -> elt),
-    M.Equal (M.mapi f (M.empty elt)) (M.empty elt).
+    Proper (O.eq ==> eq ==> eq) f
+      -> M.Equal (M.mapi f (M.empty elt)) (M.empty elt).
 Proof.
-  intros f k.
+  intros f k H.
   rewrite F.mapi_o, F.empty_o; trivial.
   intros.
-  apply Oeq_eq in H; subst.
+  rewrite H0.
   reflexivity.
 Qed.
 
@@ -107,10 +160,122 @@ Proof.
   reflexivity.
 Qed.
 
-Lemma for_all_mapi (Oeq_eq : forall a b, O.eq a b -> a = b) :
+Definition build_map_left (x : M.t elt) (k : M.key * elt) :=
+  if P (fst k) (snd k)
+  then M.add (fst k) (snd k) x
+  else x.
+
+Global Program Instance build_map_left_Proper :
+  Proper (M.Equal ==> (fun p p' => O.eq (fst p) (fst p') /\ snd p = snd p')
+                  ==> M.Equal) build_map_left.
+Obligation 1.
+  intros ???????.
+  unfold build_map_left.
+  destruct x0, y0; simpl in *.
+  destruct H0; subst.
+  rewrite H0.
+  destruct (P t0 e0).
+    rewrite H0, H.
+    reflexivity.
+  rewrite H.
+  reflexivity.
+Qed.
+
+Definition build_map_right (k : M.key * elt) (x : M.t elt) :=
+  if P (fst k) (snd k)
+  then M.add (fst k) (snd k) x
+  else x.
+
+Global Program Instance build_map_right_Proper :
+  Proper ((fun p p' => O.eq (fst p) (fst p') /\ snd p = snd p')
+            ==> M.Equal ==> M.Equal) build_map_right.
+Obligation 1.
+  intros ???????.
+  unfold build_map_right.
+  destruct x, y; simpl in *.
+  destruct H; subst.
+  rewrite H.
+  destruct (P t0 e0).
+    rewrite H0, H.
+    reflexivity.
+  rewrite H0.
+  reflexivity.
+Qed.
+
+Global Program Instance fold_left_Equal_Proper (m : list (M.key * elt)) :
+  Proper (M.Equal ==> M.Equal) (fold_left build_map_left m).
+Obligation 1.
+  intros ???; subst.
+  generalize dependent x.
+  generalize dependent y.
+  induction m; simpl; trivial.
+  destruct a; simpl.
+  destruct (P k e); simpl; intros;
+  apply IHm;
+  rewrite H;
+  reflexivity.
+Qed.
+
+Require Import Coq.Sorting.Permutation.
+
+Theorem add_transitive
+        (k : M.key) (e : elt)
+        (k0 : M.key) (e0 : elt)
+        (z : M.t elt) :
+  (O.eq k k0 -> e = e0)
+    -> M.Equal (M.add k e (M.add k0 e0 z)) (M.add k0 e0 (M.add k e z)).
+Proof.
+  intros H addr.
+  rewrite !F.add_o.
+  destruct (O.eq_dec k addr);
+  destruct (O.eq_dec k0 addr); eauto.
+  apply O.eq_sym in e2.
+  pose proof (O.eq_trans e1 e2).
+  rewrite (H H0).
+  reflexivity.
+Qed.
+
+Lemma fold_add_cons (m : list (M.key * elt)) (z : M.t elt) y :
+  (forall k e, O.eq k (fst y) -> e = snd y) ->
+  M.Equal
+    (List.fold_left
+       (fun (x : M.t elt) (k : M.key * elt) =>
+          if P (fst k) (snd k) then M.add (fst k) (snd k) x else x)
+       (y :: m) z)
+    (if P (fst y) (snd y)
+     then M.add (fst y) (snd y)
+                (List.fold_left
+                   (fun (x : M.t elt) (k : M.key * elt) =>
+                      if P (fst k) (snd k) then M.add (fst k) (snd k) x else x)
+                   m z)
+     else List.fold_left
+            (fun (x : M.t elt) (k : M.key * elt) =>
+               if P (fst k) (snd k) then M.add (fst k) (snd k) x else x)
+            m z).
+Proof.
+  intros.
+  destruct y as [k e]; simpl in *.
+  destruct (P k e); simpl.
+    generalize dependent z.
+    generalize dependent e.
+    generalize dependent k.
+    induction m; simpl.
+      reflexivity.
+    destruct a; simpl; intros.
+    rewrite <- IHm; clear IHm.
+      destruct (P k e); simpl.
+        apply fold_left_Equal_Proper, add_transitive.
+        apply H.
+      reflexivity.
+    apply H.
+  reflexivity.
+Qed.
+
+Lemma for_all_mapi :
   forall elt' (m : M.t elt') (k : M.key)
          (f : M.key -> elt' -> elt),
-    P.for_all P (M.mapi f m) = true
+    Proper (O.eq ==> eq ==> eq) f
+      -> P.for_all P (M.mapi f m) = true
       <-> P.for_all (fun k e => P k (f k e)) m = true.
 Proof.
 Abort.
@@ -152,13 +317,180 @@ Proof.
   inversion H0.
 Qed.
 
+Lemma add_equal_iff : forall elt k (e : elt) m1 m2,
+  P.Add k e m1 m2 <-> M.Equal (M.add k e m1) m2.
+Proof.
+  split; intros; intro addr;
+  specialize (H addr);
+  congruence.
+Qed.
+
+Global Program Instance fold_Proper {elt A} : forall f,
+  Proper (O.eq ==> @eq elt ==> @eq A ==> @eq A) f
+    -> P.transpose_neqkey eq f
+    -> Proper (M.Equal (elt:=elt) ==> @eq A ==> @eq A)
+              (@M.fold elt A f).
+Obligation 1.
+  intros ??????; subst.
+  revert H1.
+  revert y.
+  apply P.fold_rec; intros.
+    rewrite P.fold_Empty; auto.
+    rewrite <- H2.
+    assumption.
+  rewrite P.fold_Add; eauto.
+    apply H; auto.
+    apply H4; reflexivity.
+  congruence.
+Qed.
+
+Global Program Instance filter_Proper {elt} : forall P,
+  Proper (O.eq ==> eq ==> eq) P
+    -> Proper (M.Equal (elt:=elt) ==> M.Equal) (@P.filter elt P).
+Obligation 1.
+  intros ???; subst.
+  unfold P.filter at 1.
+  generalize dependent y.
+  apply P.fold_rec; intros.
+    apply F.Equal_mapsto_iff.
+    split; intros.
+      inversion H2.
+    apply P.filter_iff in H2; auto.
+    destruct H2.
+    rewrite <- H1 in H2.
+    apply P.elements_Empty in H0.
+    apply F.find_mapsto_iff in H2.
+    rewrite F.elements_o in H2.
+    rewrite H0 in H2.
+    inversion H2.
+  specialize (H3 m' (F.Equal_refl _)).
+  apply add_equal_iff in H2.
+  rewrite <- H2 in H4; clear H2 m'' H0.
+  destruct (P k e) eqn:Heqe; rewrite H3; clear H3.
+    apply F.Equal_mapsto_iff.
+    split; intros.
+      apply P.filter_iff; auto.
+      apply F.find_mapsto_iff in H0.
+      simplify_maps.
+        rewrite <- H4, H2.
+        intuition.
+          apply F.find_mapsto_iff.
+          rewrite F.add_eq_o; auto.
+        rewrite <- H2.
+        assumption.
+      apply F.find_mapsto_iff in H6.
+      apply P.filter_iff in H6; auto.
+      rewrite <- H4.
+      intuition.
+      apply F.find_mapsto_iff.
+      rewrite F.add_neq_o; auto.
+      apply F.find_mapsto_iff.
+      assumption.
+    apply P.filter_iff in H0; auto.
+    destruct H0.
+    rewrite <- H4 in H0.
+    apply F.find_mapsto_iff in H0.
+    simplify_maps.
+      rewrite H3.
+      apply F.find_mapsto_iff.
+      rewrite F.add_eq_o; auto.
+    apply F.find_mapsto_iff.
+    rewrite F.add_neq_o; auto.
+    apply F.find_mapsto_iff.
+    apply P.filter_iff; auto.
+    apply F.find_mapsto_iff in H7.
+    intuition.
+  apply F.Equal_mapsto_iff.
+  split; intros;
+  apply P.filter_iff in H0; auto;
+  apply P.filter_iff; auto;
+  intuition.
+    rewrite <- H4; clear H4.
+    apply F.add_neq_mapsto_iff; auto.
+    unfold not; intros.
+    rewrite <- H0 in H2.
+    apply F.not_find_in_iff in H1.
+    apply F.find_mapsto_iff in H2.
+    congruence.
+  rewrite <- H4 in H2; clear H4.
+  apply F.find_mapsto_iff in H2.
+  simplify_maps.
+    rewrite H0 in Heqe.
+    congruence.
+  apply F.find_mapsto_iff.
+  assumption.
+Qed.
+
+Lemma fold_Some_f_Proper {elt} : forall (P : M.key -> elt -> bool),
+  Proper (O.eq ==> eq ==> eq ==> eq)
+         (fun (k : M.key) (e : elt) (x0 : option (M.key * elt)) =>
+            match x0 with
+            | Some _ => x0
+            | None => if P k e then Some (k, e) else None
+            end).
+Proof.
+Admitted.
+
+Lemma fold_Some_f_negkey {elt} : forall (P : M.key -> elt -> bool),
+  P.transpose_neqkey
+    eq (fun (k : M.key) (e : elt) (x0 : option (M.key * elt)) =>
+          match x0 with
+          | Some _ => x0
+          | None => if P k e then Some (k, e) else None
+          end).
+Proof.
+Admitted.
+
+Global Program Instance find_if_Proper :
+  forall elt (P : M.key -> elt -> bool),
+    Proper (O.eq ==> eq ==> eq) P ->
+    Proper (M.Equal ==> (fun p p' =>
+                           match p, p' return Prop with
+                           | Some (k, e), Some (k', e') =>
+                             O.eq k k' /\ e = e'
+                           | None, None => True
+                           | _, _ => False
+                           end)) (find_if P).
+Obligation 1.
+  unfold find_if; intros ???.
+  pose proof
+    (fold_Proper
+       (fun (k : M.key) (e : elt) (x0 : option (M.key * elt)) =>
+          match x0 with
+          | Some _ => x0
+          | None => if P k e then Some (k, e) else None
+          end)
+       (fold_Some_f_Proper _)
+       (fold_Some_f_negkey _) x y H0).
+  erewrite H1; eauto; clear x H1 H0.
+  apply P.fold_rec; intros; auto.
+  destruct a; auto.
+  destruct (P k e); auto.
+Qed.
+
 Definition singleton {elt} (k : M.key) (e : elt) : M.t elt :=
-  P.of_list [(k, e)].
+  M.add k e (M.empty _).
 Arguments singleton {elt} k e /.
+
+Corollary MapsTo_singleton : forall k elt (e : elt),
+  M.MapsTo k e (singleton k e).
+Proof. intros; constructor; reflexivity. Qed.
 
 Corollary fold_left_singleton : forall elt k (e : elt) A (z : A) f,
   M.fold f (M.add k e (M.empty elt)) z = f k e z.
 Proof. intros; rewrite M.fold_1; reflexivity. Qed.
+
+Lemma find_if_singleton : forall elt (P : M.key -> elt -> bool) k k' e e',
+  find_if P (singleton k e) = Some (k', e')
+  -> k = k' /\ e = e' /\ P k e = true.
+Proof.
+  unfold find_if, singleton; intros.
+  rewrite M.fold_1 in H.
+  simpl in H.
+  destruct (P k e).
+    intuition; congruence.
+  discriminate.
+Qed.
 
 Lemma filter_empty : forall elt (m : M.t elt) P,
   M.Empty (elt:=elt) m -> M.Empty (elt:=elt) (P.filter P m).
@@ -257,12 +589,17 @@ Proof.
 Abort.
 
 Lemma filter_elements : forall elt (m : M.t elt) P,
-  M.elements (P.filter P m)
-    = List.filter (fun p => P (fst p) (snd p)) (M.elements m).
+  M.Equal (P.filter P m)
+          (P.of_list (List.filter (fun p => P (fst p) (snd p))
+                                  (M.elements m))).
 Proof.
-  unfold P.filter; intros.
-  Fail rewrite fold_elements.
-  induction (M.elements (elt:=elt) m); trivial.
+  intros.
+  unfold P.of_list, P.uncurry.
+  rewrite fold_right_filter.
+  unfold P.filter.
+  rewrite P.fold_spec_right.
+  unfold P.uncurry.
+  induction m using P.map_induction.
 Abort.
 
 Lemma filter_for_all : forall elt (m : M.t elt) P,
@@ -307,22 +644,22 @@ Proof.
   apply filter_idempotent; assumption.
 Qed.
 
-Lemma find_if_1 : forall elt (m : M.t elt) P,
-  find_if P m = match M.elements (P.filter P m) with
-                | [] => None
-                | x :: _ => Some x
-                end.
+Lemma add_singleton :
+  forall k k0 A (e e0 : A) m,
+    M.Equal (M.add k0 e0 m) (singleton k e) ->
+      O.eq k0 k /\ e0 = e /\ M.Empty m.
 Proof.
-  unfold find_if; intros.
-  Fail rewrite M.fold_1, filter_elements.
-  induction (M.elements (elt:=elt) m); trivial.
-  simpl filter.
-  Fail rewrite fold_Some_cons, <- surjective_pairing; auto.
-  Fail destruct (P (fst a) (snd a)); auto.
+  unfold singleton; intros.
+  induction m as [IHm|m' m'' IHm k' e' H1 H2] using P.map_induction;
+  eapply F.Equal_mapsto_iff in H;
+  destruct H as [_ H];
+  specialize (H (MapsTo_singleton k _ e));
+  apply F.find_mapsto_iff in H;
+  simplify_maps.
+  - intuition.
+  - simplify_maps.
+  - intuition.
 Abort.
-
-(* Lemma findA_nil : forall l, *)
-(*   (forall y : M.key, findA (F.eqb y) l = []) -> l = []. *)
 
 Lemma eqb_refl : forall k, F.eqb k k = true.
 Proof.
@@ -352,41 +689,75 @@ Lemma singleton_of_list : forall elt (m : M.t elt) l,
 Proof.
   intros.
   induction m using P.map_induction.
-    admit.
-  destruct l.
-    admit.
-  specialize (H0 x).
-  rewrite !F.elements_o in H0; simpl in H0.
 Abort.
 
 Lemma filter_singleton_elements : forall elt k (e : elt) m P,
-  M.Equal (P.filter P m) (singleton k e)
+  Proper (O.eq ==> eq ==> eq) P
+    -> M.Equal (P.filter P m) (singleton k e)
     -> M.elements (P.filter P m) = [(k, e)].
 Proof.
   intros.
-  induction m using P.map_induction.
-    apply filter_empty with (P:=P) in H0.
-    apply P.elements_Empty in H0.
-    specialize (H k).
-    rewrite !F.elements_o, H0 in H.
-    simpl in H; rewrite eqb_refl in H.
-    discriminate.
-  Fail apply singleton_of_list.
-    Fail constructor; constructor.
-  simpl.
-  unfold P.uncurry; simpl.
-  Fail exact H.
+  eapply F.Equal_mapsto_iff in H0.
+  destruct H0.
+  specialize (H1 (MapsTo_singleton k _ e)).
+  apply F.find_mapsto_iff in H1.
+  simplify_maps; trivial.
+  clear H0.
+  revert H2.
+  unfold P.filter.
+  apply P.fold_rec; intros.
 Abort.
 
-Lemma find_if_filter : forall elt k (e : elt) m P,
-  Proper (O.eq ==> eq ==> eq) P
-    -> M.Equal (P.filter P m) (singleton k e)
-    -> find_if P m = Some (k, e).
+Lemma equal_add :
+  forall k0 k elt (e0 e : elt) m,
+    M.Equal (M.add k0 e0 m) (M.add k e (M.empty elt))
+      -> (O.eq k k0 /\ e0 = e) \/ M.Equal m (M.empty elt).
 Proof.
-  unfold singleton; intros.
-  Fail rewrite find_if_1.
-  Fail rewrite (filter_singleton_elements _ _ _ _ _ H0).
-  Fail reflexivity.
+  intros.
+  destruct (O.eq_dec k k0).
+  - left.
+    specialize (H k0).
+    rewrite !F.add_o in H.
+    destruct (O.eq_dec k0 k0);
+    destruct (O.eq_dec k k0).
+    + inversion H; subst.
+      intuition.
+    + intuition.
+    + contradiction n.
+      reflexivity.
+    + contradiction.
+  - right.
+Abort.
+
+Lemma find_if_filter : forall elt (m : M.t elt) P,
+  Proper (O.eq ==> eq ==> eq) P
+    -> find_if P (P.filter P m) = find_if P m.
+Proof.
+  intros.
+Admitted.
+
+Lemma find_if_filter_is_singleton :
+  forall elt k (e : elt) m P,
+    Proper (O.eq ==> eq ==> eq) P
+      -> M.Equal (P.filter P m) (singleton k e)
+      -> find_if P m = Some (k, e).
+Proof.
+  intros.
+  rewrite <- find_if_filter.
+  pose proof (find_if_Proper
+                _ P H (P.filter P m) (singleton k e) H0).
+  simpl in H1.
+  destruct (find_if P (P.filter P m)) eqn:Heqe1.
+    destruct p.
+    destruct (find_if P (M.add k e (M.empty elt))) eqn:Heqe2.
+      destruct p.
+      pose proof (find_if_singleton _ P _ _ _ _ Heqe2).
+      intuition; subst.
+      rewrite <- Heqe1, <- Heqe2.
+      admit.
+  rewrite H0.
+  unfold find_if; intros.
+  
 Abort.
 
 End FMapExt.
